WIP

iris_system/IModL.v
@@ -10,13 +10,14 @@ Require Export IPM.
 
 Section ILIST.
   Context `{Σ: GRA.t}.
+  Notation iProp := (iProp Σ).
 
   Definition iPropL := alist string iProp.
 
   Fixpoint from_iPropL (l: iPropL): iProp :=
     match l with
     | [] => (emp)%I
-    | (_, Phd)::Ptl => Phd ** (from_iPropL Ptl)
+    | (_, Phd)::Ptl => Phd ∗ (from_iPropL Ptl)
     end.
 
   Fixpoint get_ipm_pat (l: iPropL): string :=
@@ -87,11 +88,12 @@ Section ILIST.
   Lemma iPropL_find_remove (Hn: string) (l: iPropL) P
         (FIND: alist_find Hn l = Some P)
     :
-      from_iPropL l -∗ #=> (P ** from_iPropL (alist_remove Hn l)).
+      from_iPropL l -∗ #=> (P ∗ from_iPropL (alist_remove Hn l)).
   Proof.
     revert P FIND. induction l; ss. i.
     destruct a. iIntros "[H0 H1]".
-    rewrite eq_rel_dec_correct in *. des_ifs; ss.
+    rewrite eq_rel_dec_correct in FIND.
+    rewrite eq_rel_dec_correct. des_ifs; ss.
     { iPoseProof (IHl with "H1") as "> H1"; et.
       iModIntro. iFrame. iFrame. }
     { iFrame. iApply iPropL_clear. iFrame. }
@@ -120,7 +122,8 @@ Section ILIST.
   Proof.
     revert P0 P1 FIND ENTAIL. induction l; ss. i.
     destruct a. iIntros "[H0 H1]".
-    rewrite eq_rel_dec_correct in *. des_ifs.
+    rewrite eq_rel_dec_correct in FIND.
+    rewrite eq_rel_dec_correct. des_ifs.
     { ss. iPoseProof (IHl with "H1") as "H1"; et. repeat iFrame. }
     { ss. iPoseProof (ENTAIL with "H0") as "> H0".
       iPoseProof (iPropL_clear with "H1") as "> H1".
@@ -152,7 +155,8 @@ Section ILIST.
   Proof.
     revert FIND. induction l; ss. i.
     destruct a. iIntros "[H0 H1]".
-    rewrite eq_rel_dec_correct in *. des_ifs; ss.
+    rewrite eq_rel_dec_correct in FIND.
+    rewrite eq_rel_dec_correct. des_ifs; ss.
     { iPoseProof (IHl with "H1") as (a) "H1"; et.
       iExists a. repeat iFrame. }
     { iDestruct "H0" as (a) "H0". iExists a.
@@ -166,7 +170,8 @@ Section ILIST.
   Proof.
     revert FIND. induction l; ss. i.
     destruct a. iIntros "[H0 H1]".
-    rewrite eq_rel_dec_correct in *. des_ifs; ss.
+    rewrite eq_rel_dec_correct in FIND.
+    rewrite eq_rel_dec_correct. des_ifs; ss.
     { iPoseProof (IHl with "H1") as "[H1|H1]"; et.
       { iLeft. repeat iFrame. }
       { iRight. repeat iFrame. }
@@ -179,14 +184,14 @@ Section ILIST.
 
   Lemma iPropL_add (Hn: string) (l: iPropL) P
     :
-      P ** from_iPropL l -∗ #=> (from_iPropL (alist_add Hn P l)).
+      P ∗ from_iPropL l -∗ #=> (from_iPropL (alist_add Hn P l)).
   Proof.
     unfold alist_add. ss. iIntros "[H0 H1]".
     iFrame. iApply iPropL_clear. iFrame.
   Qed.
 
   Lemma iPropL_destruct_sep Hn_old Hn_new0 Hn_new1 (l: iPropL) (P0 P1: iProp)
-        (FIND: alist_find Hn_old l = Some (P0 ** P1))
+        (FIND: alist_find Hn_old l = Some (P0 ∗ P1)%I)
     :
       from_iPropL l -∗ #=> from_iPropL (alist_add Hn_new1 P1 (alist_add Hn_new0 P0 (alist_remove Hn_old l))).
   Proof.
@@ -200,17 +205,17 @@ Section ILIST.
   Lemma iPropL_alist_pop Hn P (l0 l1: iPropL)
         (FIND: alist_pop Hn l0 = Some (P, l1))
     :
-      from_iPropL l0 ⊢ P ** from_iPropL l1.
+      from_iPropL l0 ⊢ P ∗ from_iPropL l1.
   Proof.
     revert P l1 FIND. induction l0; ss. i.
-    destruct a. rewrite eq_rel_dec_correct in *. des_ifs.
+    destruct a. rewrite eq_rel_dec_correct in FIND. des_ifs.
     ss. hexploit IHl0; et. i.
     iIntros "[H0 H1]". iFrame. iApply H. iFrame.
   Qed.
 
   Lemma iPropL_alist_pops l Hns
     :
-      from_iPropL l ⊢ from_iPropL (fst (alist_pops Hns l)) ** from_iPropL (snd (alist_pops Hns l)).
+      from_iPropL l ⊢ from_iPropL (fst (alist_pops Hns l)) ∗ from_iPropL (snd (alist_pops Hns l)).
   Proof.
     induction Hns. ss.
     { iIntros "H0". iFrame. }
@@ -270,38 +275,38 @@ Section IMOD.
     (λ x : A, x0 <- Ret x;; k x0) = k.
   Proof. extensionality x. grind. Qed.
 
-  Lemma imod_trans `{Σ: GRA.t} (P Q R: iProp) :
+  Lemma imod_trans `{Σ: GRA.t} (P Q R: iProp Σ) :
     (P ⊢ #=> Q) -> (Q ⊢ #=> R) -> (P ⊢ #=> R).
   Proof.
-    i. iIntros "H". iPoseProof (H with "H") as "H". iMod "H".
-    iPoseProof (H0 with "H") as "H". eauto.
+    etransitivity; eauto.
+    iIntros ">Q". by iApply H0.
   Qed.
 
-  Lemma imod_elim_trueL `{Σ: GRA.t} P Q :
-    (P ⊢ #=> Q) -> (P ⊢ #=> (True ** Q)).
+  Lemma imod_elim_trueL `{Σ: GRA.t} (P Q : iProp Σ) :
+    (P ⊢ #=> Q) -> (P ⊢ #=> (True ∗ Q)).
   Proof.
     i. iIntros "H". iSplitR; eauto. iStopProof. eauto.
-  Qed.  
+  Qed.
 
-  Lemma imod_intro_trueL `{Σ: GRA.t} P Q :
-    (P ⊢ #=> (True ** Q)) -> (P ⊢ #=> Q).
+  Lemma imod_intro_trueL `{Σ: GRA.t} (P Q : iProp Σ) :
+    (P ⊢ #=> (True ∗ Q)) -> (P ⊢ #=> Q).
   Proof.
     i. iIntros "H". iPoseProof (H with "H") as "H".
     iMod "H". iDestruct "H" as "[X Y]". eauto.
-  Qed.  
+  Qed.
 
-  Lemma imod_elim_trueR `{Σ: GRA.t} P Q :
-    (P ⊢ #=> Q) -> (P ⊢ #=> (Q ** True)).
+  Lemma imod_elim_trueR `{Σ: GRA.t} (P Q : iProp Σ) :
+    (P ⊢ #=> Q) -> (P ⊢ #=> (Q ∗ True)).
   Proof.
     i. iIntros "H". iSplitL; eauto. iStopProof. eauto.
-  Qed.  
+  Qed.
 
-  Lemma imod_intro_trueR `{Σ: GRA.t} P Q :
-    (P ⊢ #=> (Q ** True)) -> (P ⊢ #=> Q).
+  Lemma imod_intro_trueR `{Σ: GRA.t} (P Q : iProp Σ) :
+    (P ⊢ #=> (Q ∗ True)) -> (P ⊢ #=> Q).
   Proof.
     i. iIntros "H". iPoseProof (H with "H") as "H".
     iMod "H". iDestruct "H" as "[X Y]". eauto.
-  Qed.  
+  Qed.
 End IMOD.
 
 Create HintDb imodL.
@@ -309,12 +314,12 @@ Hint Resolve imod_trans imod_elim_trueL: imodL.
 
 
 Ltac imodIntroL :=
-  i; repeat match goal with [H: (_ ⊢ #=> (True ** _)) |- _ ] => apply imod_intro_trueL in H end; eauto with imodL.
-  
+  i; repeat match goal with [H: (_ ⊢ #=> (True ∗ _)) |- _ ] => apply imod_intro_trueL in H end; eauto with imodL.
+
 Ltac grind_ret := try rewrite !bind_ret_l_eta in *; subst.
 
 Ltac itree_clarify H :=
-  revert H; grind; try unfold trigger in H; try rewrite !bind_vis in H; try depdes H; grind_ret. 
+  revert H; grind; try unfold trigger in H; try rewrite !bind_vis in H; try depdes H; grind_ret.
 
 
 
