lib/Axioms.v
@@ -1,5 +1,7 @@
 Require ClassicalFacts.
 Require FunctionalExtensionality.
+Require ChoiceFacts.
+Require IndefiniteDescription.
 
 Lemma func_ext_dep {A} {B: A -> Type} (f g: forall x, B x): (forall x, f x = g x) -> f = g.
 Proof.
@@ -9,6 +11,15 @@ Qed.
 Lemma func_ext {A B} (f g: A -> B): (forall x, f x = g x) -> f = g.
 Proof.
   apply func_ext_dep.
+Qed.
+
+Lemma dependent_functional_choice {A : Type} (B : A -> Type) :
+  forall R : forall x : A, B x -> Prop,
+    (forall x : A, exists y : B x, R x y) ->
+    (exists f : (forall x : A, B x), forall x : A, R x (f x)).
+Proof.
+  eapply ChoiceFacts.non_dep_dep_functional_choice.
+  clear. exact Coq.Logic.IndefiniteDescription.functional_choice.
 Qed.
 
 Axiom proof_irr: ClassicalFacts.proof_irrelevance.
